theories/base_logic/lib/cancelable_invariants.v
@@ -93,12 +93,12 @@ Section proofs.
 
   Global Instance into_inv_cinv N γ P : IntoInv (cinv N γ P) N.
   Global Instance elim_inv_cinv p γ E N P Q Q' :
-    (∀ R, ElimModal True (|={E,E∖↑N}=> R) R Q Q') →
+    (∀ R, ElimModal True false false (|={E,E∖↑N}=> R) R Q Q') →
     ElimInv (↑N ⊆ E) (cinv N γ P) (cinv_own γ p)
       (▷ P ∗ cinv_own γ p) (▷ P ={E∖↑N,E}=∗ True) Q Q'.
   Proof.
     rewrite /ElimInv /ElimModal. iIntros (Helim ?) "(#H1&Hown&H2)".
-    iApply Helim; [done|]. iSplitR "H2"; [|done].
+    iApply Helim; [done|]; simpl. iSplitR "H2"; [|done].
     iMod (cinv_open E N γ p P with "[#] [Hown]") as "(HP&Hown&Hclose)"; auto. 
     by iFrame.
   Qed.
